\subsubsection*{FLGV}
According to \textbf{FLGV-2}, we have:
\[\exists \textbf{y} \in \textbb{R}^{m}: A^{T}\textbf{y} \geq 0, \textbf{b}^{T}\textbf{y} < 0 \]
if FLGV-1 also holds, there exists $\textbf{x} \geq 0$, $A\textbf{x}=\textbf{b}$.
\noindent
because $A\textbf{x}=\textbf{b}$ can be written as $\textbf{b}^{T} = \textbf{x}^{T}A^{T}$, we have:
\[\textbf{b}^{T}\textbf{y}=\textbf{x}^{T}A^{T}\textbf{y}\]
Because $A^{T}\textbf{y} \geq 0$, $\textbf{x} \geq 0$, we can get $\textbf{x}^{T}A^{T}\textbf{y} \geq 0$. But according to \textbf{FLGV-2}, $\textbf{b}^{T}\textbf{y} < 0$, which is a contradictory, so FLGV-2 implies that \textbf{FLGV-1} does not hold.
\subsubsection*{FLLPV}
According to \textbf{FLLPV-2}, we have:
\[\exists \textbf{y} \in \mathbb{R}^{m}: \textbf{y} \geq 0, A^{T}\textbf{y} \geq 0, \textbf{b}^{T}\textbf{y} < 0 \]
if \textbf{FLLPV-1} also holds, there exists $\textbf{x} \geq 0$, $A\textbf{x} \leq \textbf{b}$. Because $A\textbf{x} \leq \textbf{b}$ can be written as $\textbf{b}^{T} \geq \textbf{x}^{T}A^{T}$, and $\textbf{y}$ holds $\textbf{y} \geq 0$, we have:
\[\textbf{b}^{T}\textbf{y} \geq \textbf{x}^{T}A^{T}\textbf{y}\]
Because $A^{T}\textbf{y} \geq 0$, $\textbf{x} \geq 0$, we can get $\textbf{b}^{T}\textbf{y} \geq \textbf{x}^{T}A^{T}\textbf{y} \geq 0$.
But according to \textbf{FLLPV-2}, $\textbf{b}^{T}\textbf{y} < 0$, which is a contradictory, so \textbf{FLLPV-2} implies that FLLPV-1 does not hold.
\subsubsection*{FLEV}
According to \textbf{FLEV-2}, we have:
\[\exists \textbf{y} \in \mathbb{R}^{m}: \textbf{y} \geq 0, A^{T}\textbf{y} \geq 0, \textbf{b}^{T}\textbf{y} < 0 \]
If \textbf{FLEV-1} also holds, there exists $A\textbf{x} \leq \textbf{b}$.
Because $A\textbf{x} \leq \textbf{b}$ can be written as $\textbf{b}^{T} \geq \textbf{x}^{T}A^{T}$, and $\textbf{y}$ holds $\textbf{y} \geq 0$, we have:
\[\textbf{b}^{T}\textbf{y} \geq \textbf{x}^{T}A^{T}\textbf{y}\]
Because $A^{T}\textbf{y} \geq 0$, $\textbf{x} \geq 0$, we can get $\textbf{b}^{T}\textbf{y} \geq \textbf{x}^{T}A^{T}\textbf{y} \geq 0$.
But according to \textbf{FLEV-2}, $\textbf{b}^{T}\textbf{y} < 0$, which is a contradictory, so \textbf{FLEV-2} implies that FLEV-1 does not hold.
