        We need to calculate the fomula in Ex8 for a random $A$ and a specific $k$. 
		
		\begin{align*}
			\mathbb{E}[C]&= \sum_{i = 1}^{n}\sum_{j = 1}^{n} \mathbb{E}[B_{i,j,k}] - \mathbb{E}[k\text{~is~a~leaf}]\\
				&= \sum_{i \neq j} \mathbb{E}[B_{i,j,k}] + \sum_{i = 1}^{n} \mathbb{E}[B_{i,i,k}] - \mathbb{E}[k\text{~is~a~leaf}]\\
				&= 2\sum_{1 \leq i < j \leq n} \mathbb{E}[B_{i,j,k}] + \sum_{i = 1}^{n} \mathbb{E}[A_{i,k}] - \mathbb{E}[k\text{~is~a~leaf}]
		\end{align*}
		
		Firstly, we calculate$\displaystyle \sum_{1 \leq i < j \leq n} \mathbb{E}[B_{i,j,k}]$
        \begin{itemize}
        \item When $k\leq i$ holds:
        \begin{align*}
        \sum_{k\leq i<j}\mathbb{E}[B_{i,j,k}]&=\sum_{k<j}\frac{\binom{1}{j-k}}{j-k+1}\\
        &=\sum_{\Delta=1}^{n-k}\frac{\Delta}{\Delta+1}\\
        &=\sum_{\Delta=1}^{n-k}(1-\frac{1}{\Delta+1})\\
        &=n-k-H_{n-k+1}+1
        \end{align*}
        \item When $j\leq k$ holds:
        \begin{align*}
        \sum_{i<j\leq k}\mathbb{E}[B_{i,j,k}]&=\sum_{i<k}\frac{\binom{1}{k-i}}{k-i+1}\\
        &=\sum_{\Delta=1}^{k-1}\frac{\Delta}{\Delta+1}\\
        &=\sum_{\Delta=1}^{k-1}(1-\frac{1}{\Delta+1})\\
        &=k-H_{k}
        \end{align*}
        \item When $i<k$ and $k<j$ holds:
        \begin{align*}
        \sum_{i<k<j}\mathbb{E}[B_{i,j,k}] &= \sum_{i = 1}^{k - 1} \sum_{j = k + 1}^{n} \frac{1}{j - i + 1}\\
        &= \sum_{i = 1}^{k - 1} \sum_{t = k - i + 2}^{n - i + 1} \frac{1}{t}\\
        &= \sum_{i = 1}^{k - 1} (\sum_{t = 3}^{n} \frac{1}{t} - \sum_{t = 3}^{k - i + 1} \frac{1}{t} - \sum_{t = n - i + 2}^{n} \frac{1}{t})\\
        &= \sum_{i = 1}^{k - 1}(H_n - H_2) - \sum_{i = 1}^{k - 1} \sum_{t = 3}^{k - i + 1} \frac{1}{t} - \sum_{i = 1}^{k - 1} \sum_{t = n - i + 2}^{n} \frac{1}{t}\\
        &= (k - 1)(H_n - H_2) - \sum_{t = 3}^{k} \sum_{i = 1}^{k - t + 1} \frac{1}{t} - \sum_{t = n - k + 3}^{n} \sum_{i = n - t + 2}^{k - 1} \frac{1}{t}\\
        &= (k - 1)(H_n - H_2) - \sum_{t = 3}^{k} \frac{k - t + 1}{t} - \sum_{t = n - k + 3}^{n} \frac{t + k - n - 2}{t}\\
        &= (k - 1)(H_n - H_2) - \sum_{t = 3}^{k} (\frac{k + 1}{t} - 1) - \sum_{t = n - k + 3}^{n} (\frac{k - n - 2}{t} + 1)\\
        &= (k - 1)(H_n - H_2) - (k + 1)\sum_{t = 3}^{k} \frac{1}{t} + (k - 2) \\
		&~~~-(k - n - 2) \sum_{t = n - k + 3}^{n} \frac{1}{t} - (k - 2)\\
        &= (k - 1)(H_n - H_2) - (k + 1)(H_k - H_2) - (k - n - 2)(H_n - H_{n - k + 2})\\
        &= (n + 1)H_n - (k + 1)H_k - (n - k + 2)H_{n - k + 2} + 3
        \end{align*}
        \end{itemize}
        Then we have:
        \begin{align*}
        \sum_{1 \leq i < j \leq n} \mathbb{E}[B_{i,j,k}]&=\sum_{k\leq i<j}\mathbb{E}[B_{i,j,k}] + \sum_{i<j\leq k}\mathbb{E}[B_{i,j,k}] + \sum_{i<k<j}\mathbb{E}[B_{i,j,k}]\\
			&=n-k-H_{n-k+1}+1+k-H_{k}+(n + 1)H_n - (k + 1)H_k\\
			&~~~- (n - k + 2)H_{n - k + 2} + 3\\
			&=n-(n-k+3)H_{n-k+1}+(n+1)H_n-(k+2)H_{k}+3
        \end{align*}
		
		Secondly, we calculate $\displaystyle \sum_{i = 1}^{n} \mathbb{E}[A_{i,k}]$
		 \begin{align*}
			\sum_{i = 1}^{n} \mathbb{E}[A_{i,k}] &= \sum_{i = 1}^{n} \frac{1}{|i - k| + 1}\\
										&= \sum_{i = 1}^{k} \frac{1}{k - i + 1} + \sum_{i = k + 1}^{n} \frac{1}{i - k + 1}\\
										&= \sum_{t = 1}^{k} \frac{1}{t} + \sum_{t = 2}^{n - k + 1} \frac{1}{t}\\
										&= H_k + H_{n - k + 1} - 1
		 \end{align*}
		 
		 Thirdly, we calculate $\displaystyle \mathbb{E}[k\text{~is~a~leaf}]$
		 $k$ is a leaf if and only if $k - 1$ and $k + 1$(if they exist) occur before k. So
		 \[
			\mathbb{E}[k\text{~is~a~leaf}] = 
			\begin{cases}
				1 & n = 1,\\
				\frac{1}{2} &n \neq 1~\text{and}~(k = 1 or k = n),\\
				\frac{1}{3} &n \neq 1~\text{and}~1 < k < n.
			\end{cases}
		 \]
		 Totally, we get
		 \begin{align*}
			\mathbb{E}[C]	&= 2\sum_{1 \leq i < j \leq n} \mathbb{E}[B_{i,j,k}] + \sum_{i = 1}^{n} \mathbb{E}[A_{i,k}] - \mathbb{E}[k\text{~is~a~leaf}]\\
							&= 2(n-(n-k+3)H_{n-k+1}+(n+1)H_n-(k+2)H_{k}+3) + H_k + H_{n - k + 1} - 1 + \mathbb{E}[k\text{~is~a~leaf}]\\
							&=
							\begin{cases}
								0 & n = 1,\\
								2n + 2(n + 1)H_n - (2n - 2k + 5)H_{n - k + 1} - (2k + 3)H_k + 5 - \frac{1}{2} &n \neq 1~\text{and}~(k = 1 or k = n),\\
								2n + 2(n + 1)H_n - (2n - 2k + 5)H_{n - k + 1} - (2k + 3)H_k + 5 - \frac{1}{3} &n \neq 1~\text{and}~1 < k < n.
							\end{cases}
		\end{align*}