Recalling the proof that $A_{i, j} = 1$ iff the number in $[i, j]$ in the input sequence that occurs first must be $i$, we can obvirusly make an inferrence that $B_{i, j, k} = 1$ iff the number in $[i, j] \cup [i, k]$ in the input sequence that occurs first must be $i$.

Notice that every number has no difference among other numbers except their pronunciations. In other words, we can choose the number which occurs first with equal probability.

Hence
\[\mathbb{E}[B_{i, j, k}] = \dfrac{1}{\left|[i, j] \cup [i, k]\right|}\]

\begin{lemma}
$\left|[i, j] \cup [i, k]\right| = \max\{i, j, k\} - \min\{i, j, k\} + 1$
\end{lemma}
\begin{proof}
We will prove the lemma with three cases below.
\begin{itemize}
\item If $i = \min\{i, j, k\}$, then
\[\left|[i, j] \cup [i, k]\right| = \max\{j, k\} - i + 1 = \max\{i, j, k\} - \min\{i, j, k\} + 1\]
\item If $i = \max\{i, j, k\}$, then
\[\left|[i, j] \cup [i, k]\right| = i - \min\{j, k\} + 1 = \max\{i, j, k\} - \min\{i, j, k\} + 1\]
\item If $j < i < k$ or $k < i < j$, then
\[\left|[i, j] \cup [i, k]\right| = \max\{j, k\} - \min\{j, k\} + 1 = \max\{i, j, k\} - \min\{i, j, k\} + 1\]
\end{itemize}
\end{proof}

According to the lemma, the following formula holds.
\[\mathbb{E}[B_{i, j, k}] = \dfrac{1}{\max\{i, j, k\} - \min\{i, j, k\} + 1}\]
